refactor: simplify relation and function defs

Set/Functions.lean
@@ -2,9 +2,8 @@ import Set.Relations
 
 namespace Set
   -- Function [Enderton, p.42]
-  def IsFunction (F A B : Set) (prop : Set → Set → Prop) : Prop :=
-    F = Relation A B prop ∧ ∀ x, x ∈ (dom F) → ∃! y, ⟨x, y⟩ ∈ F
-
+  def IsFunction (F : Set) : Prop :=
+    IsRelation F ∧ ∀ x, x ∈ (dom F) → ∃! y, ⟨x, y⟩ ∈ F
   -- A set R is single-rooted iff for each y ∈ ran R there is only one x such that xRy.
   def SingleRooted (R : Set) : Prop :=
     ∀ (y : Set), y ∈ (ran R) → ∃! (x: Set), ⟨x, y⟩ ∈ R
@@ -44,7 +43,7 @@ namespace Set
   [Enderton, Theorem 3E, p. 46]
   For a set F, dom F⁻¹ = ran F and ran F⁻¹ = dom F. For a relation F, (F⁻¹)⁻¹ = F.
   -/
-  theorem domain_range_inverse (F : Set) : (dom (Inverse F)) = ran F := by
+  theorem domain_inverse (F : Set) : (dom (Inverse F)) = ran F := by
     apply extensionality
     intro x
     apply Iff.intro
@@ -57,353 +56,74 @@ namespace Set
       aesop
     }
     { aesop }
-  theorem relation_inverse_inverse {A B : Set} {prop : Set → Set → Prop} (R : Set) :
-    R = Relation A B prop → (Inverse (Inverse R)) = R := by
-    intro h
+  theorem range_inverse (F : Set) : (ran (Inverse F)) = dom F := by
     apply extensionality
     intro x
     apply Iff.intro
-    { intro heq
-      rw [Inverse.Spec] at heq
-      obtain ⟨u, v, hu⟩ := heq
-      obtain ⟨hu₁, hu₂⟩ := hu
-      rw [Inverse.Spec] at hu₁
-      obtain ⟨v', u', hvu'⟩ := hu₁
-      rw [OrderedPair.uniqueness] at hvu'
+    { intro h
+      rw [Relation.Range.Spec] at h
+      obtain ⟨y, hy⟩ := h
+      rw [Inverse.Spec] at hy
+      obtain ⟨u, v, hu⟩ := hy
+      rw [OrderedPair.uniqueness] at hu
       aesop
     }
-    { intro heq
-      rw [Inverse.Spec]
-      rw [h] at heq
-      rw [Relation.Spec] at heq
-      obtain ⟨heq₁, heq₂⟩ := heq
-      rw [Product.Spec] at heq₁
-      obtain ⟨_, heq₁⟩ := heq₁
-      obtain ⟨u, v, hu, hv, huv⟩ := heq₁
-      apply Exists.intro v
-      apply Exists.intro u
-      apply And.intro
-      { rw [Inverse.Spec]
-        apply Exists.intro u
-        apply Exists.intro v
-        apply And.intro
-        { aesop }
-        { aesop }
-      }
-      { exact huv }
+    { aesop }
+  theorem relation_inverse_inverse (F : Set) {hF : IsRelation F} : (Inverse (Inverse F)) = F := by
+    apply extensionality
+    intro x
+    apply Iff.intro
+    { intro hx
+      rw [Inverse.Spec] at hx
+      obtain ⟨u, v, ⟨huv, huvx⟩⟩ := hx
+      rw [Inverse.Spec] at huv
+      obtain ⟨u', v', ⟨huv', huvx'⟩⟩ := huv
+      subst huvx
+      have heq : u = v' ∧ v = u' := by
+        rw [OrderedPair.uniqueness] at huvx'
+        exact huvx'
+      rw [heq.left, heq.right]
+      exact huv'
+    }
+    { intro hx
+      have huv : ∃ u v, x = ⟨u, v⟩ := by aesop
+      aesop
     }
 
-  protected lemma function_dom {F A B : Set} {prop : Set → Set → Prop} (hF : F.IsFunction A B prop) :
-    ∀ x, x ∈ (dom F) → x ∈ A := by
-    intro x hx
-    rw [IsFunction] at hF
-    obtain ⟨hF, _⟩ := hF
-    rw [Relation.Domain.Spec] at hx
-    obtain ⟨x', hx'⟩ := hx
-    rw [hF, Relation.Spec] at hx'
-    obtain ⟨hx', _⟩ := hx'
-    rw [Product.Spec] at hx'
-    obtain ⟨_, hx'⟩ := hx'
-    obtain ⟨u, v, hu, hv, heq⟩ := hx'
-    rw [OrderedPair.uniqueness] at heq
-    rw [←heq.left] at hu
-    exact hu
-
-  protected lemma function_ran {F A B : Set} {prop : Set → Set → Prop} (hF : F.IsFunction A B prop) :
-    ∀ x, x ∈ (ran F) → x ∈ B := by
-    intro x hx
-    rw [IsFunction] at hF
-    obtain ⟨hF, _⟩ := hF
-    rw [Relation.Range.Spec] at hx
-    obtain ⟨x', hx'⟩ := hx
-    rw [hF, Relation.Spec] at hx'
-    obtain ⟨hx', _⟩ := hx'
-    rw [Product.Spec] at hx'
-    obtain ⟨_, hx'⟩ := hx'
-    obtain ⟨u, v, hu, hv, heq⟩ := hx'
-    rw [OrderedPair.uniqueness] at heq
-    rw [←heq.right] at hv
-    exact hv
-
-  protected lemma function_functional
-    {F A B : Set} {prop : Set → Set → Prop} {hF : F.IsFunction A B prop} {x y y' : Set}
-    (hxy : ⟨x, y⟩ ∈ F) (hxy' : ⟨x, y'⟩ ∈ F) : y = y' := by
-    rw [IsFunction] at hF
-    obtain ⟨hF₁, hF₂⟩ := hF
-    have hx : x ∈ (dom F) := by
-      rw [Relation.Domain.Spec]
-      apply Exists.intro y
-      exact hxy
-    have huniq : ∃! y, ⟨x, y⟩ ∈ F := hF₂ x hx
-    obtain ⟨u, hu, huniq⟩ := huniq
-    have hy : y = u := by
-      apply huniq
-      exact hxy
-    have hy' : y' = u := by
-      apply huniq
-      exact hxy'
-    subst hy
-    subst hy'
-    trivial
 
   /-
-  [Enderton, Theorem 3H, p. 47]
-  Assume that F and G are functions. Then F ∘ G is a function, its domain is
-    {x ∈ dom G | G(x) ∈ dom F},
-  and for each x in its domain, (F ∘ G)(x) = F(G(x)).
+  [Enderton, Theorem 3F, p. 46]
+  For a set F, F⁻¹ is a function iff F is single-rooted. A relation F is a function iff F⁻¹ is single-rooted.
   -/
-  theorem function_composition_creates_function {F G A B C : Set} {prop₁ prop₂ : Set → Set → Prop}
-    {hF : F.IsFunction B C prop₁} {hG : G.IsFunction A B prop₂} :
-    (F ∘ G).IsFunction A C (λ u v ↦ ∃ t, t ∈ B ∧ prop₂ u t ∧ prop₁ t v) := by
-    rw [IsFunction]
-    apply And.intro
-    { apply extensionality
-      intro xy
-      apply Iff.intro
-      { intro h
-        rw [Composition.Spec] at h
-        rw [Relation.Spec]
-        obtain ⟨h₁, u, v, t, hu, ht, hv⟩ := h
-        apply And.intro
-        { -- We can show that (dom G) ⨯ (ran F) ⊆ A ⨯ C
-          have hsub : ((dom G) ⨯ (ran F)) ⊆ A ⨯ C := by
-            rw [SubsetOf]
-            intro t ht
-            rw [Product.Spec] at ht
-            obtain ⟨_, ht⟩ := ht
-            obtain ⟨x', y', hx', hy', heq⟩ := ht
-            rw [heq, Product.Spec]
-            apply And.intro
-            { apply OrderedPair.in_power_power
-              rw [Union.Spec]
-              apply Or.intro_left
-              exact Set.function_dom hG x' hx'
-              rw [Union.Spec]
-              apply Or.intro_right
-              exact Set.function_ran hF y' hy'
-            }
-            { apply Exists.intro x'
-              apply Exists.intro y'
-              apply And.intro
-              { exact Set.function_dom hG x' hx' }
-              apply And.intro
-              { apply Set.function_ran hF y' hy' }
-              { trivial }
-            }
-          rw [SubsetOf] at hsub
-          apply hsub
-          exact h₁
-        }
-        { rw [Set.relation_condition]
-          apply Exists.intro u
-          apply Exists.intro v
-          have h₁ : u ∈ A := by
-            rw [IsFunction] at hG
-            obtain ⟨hG, _⟩ := hG
-            rw [hG, Relation.Spec] at hu
-            obtain ⟨_, hu⟩ := hu
-            rw [Set.relation_condition] at hu
-            obtain ⟨u', _, hu', _, _, hut⟩ := hu
-            rw [OrderedPair.uniqueness] at hut
-            rw [←hut.left] at hu'
-            exact hu'
-          have h₂ : v ∈ C := by
-            rw [IsFunction] at hF
-            obtain ⟨hF, _⟩ := hF
-            rw [hF, Relation.Spec] at ht
-            obtain ⟨_, ht⟩ := ht
-            rw [Set.relation_condition] at ht
-            obtain ⟨_, v', _, hv', _, htv⟩ := ht
-            rw [OrderedPair.uniqueness] at htv
-            rw [←htv.right] at hv'
-            exact hv'
-          have h₃ : ∃ t, t ∈ B ∧ prop₂ u t ∧ prop₁ t v := by
-            apply Exists.intro t
-            apply And.intro
-            { rw [IsFunction] at hG
-              obtain ⟨hG, _⟩ := hG
-              rw [hG, Relation.Spec] at hu
-              obtain ⟨hu, _⟩ := hu
-              rw [Product.Spec] at hu
-              obtain ⟨_, hu⟩ := hu
-              obtain ⟨u', t', hu', ht', heq⟩ := hu
-              rw [OrderedPair.uniqueness] at heq
-              rw [←heq.right] at ht'
-              exact ht'
-            }
-            apply And.intro
-            { rw [IsFunction] at hG
-              obtain ⟨hG, _⟩ := hG
-              rw [hG, Relation.Spec] at hu
-              obtain ⟨_, hu⟩ := hu
-              rw [Set.relation_condition] at hu
-              obtain ⟨u', v', hu', hv', hprop, heq⟩ := hu
-              rw [OrderedPair.uniqueness] at heq
-              rw [←heq.left, ←heq.right] at hprop
-              exact hprop
-            }
-            { rw [IsFunction] at hF
-              obtain ⟨hF, _⟩ := hF
-              rw [hF, Relation.Spec] at ht
-              obtain ⟨_, ht⟩ := ht
-              rw [Set.relation_condition] at ht
-              obtain ⟨t', v', ht', hv', hprop, heq⟩ := ht
-              rw [OrderedPair.uniqueness] at heq
-              rw [←heq.left, ←heq.right] at hprop
-              exact hprop
-            }
-          apply And.intro h₁
-          apply And.intro h₂
-          apply And.intro h₃
-          exact hv
-        }
-      }
-      { intro h
-        rw [Composition.Spec]
-        apply And.intro
-        { rw [Product.Spec]
-          rw [Relation.Spec] at h
-          obtain ⟨h₁, h₂⟩ := h
-          apply And.intro
-          rw [Product.Spec] at h₁
-          obtain ⟨h₁, ⟨x, y, hx, hy, hxy⟩⟩ := h₁
-          { subst hxy
-            simp [Power.Spec, SubsetOf] at h₁
-            apply OrderedPair.in_power_power
-            { rw [Union.Spec]
-              apply Or.intro_left
-              rw [Relation.Domain.Spec]
-              rw [Set.relation_condition] at h₂
-              rw [IsFunction] at hG
-              obtain ⟨hG, _⟩ := hG
-              obtain ⟨x', y', _, _, ⟨t, ht⟩, heq⟩ := h₂
-              rw [OrderedPair.uniqueness] at heq
-              rw [←heq.left, ←heq.right] at ht
-              apply Exists.intro t
-              rw [hG, Relation.Spec]
-              apply And.intro
-              { rw [Product.Spec]
-                apply And.intro
-                { apply OrderedPair.in_power_power
-                  rw [Union.Spec]
-                  apply Or.intro_left
-                  exact hx
-                  rw [Union.Spec]
-                  apply Or.intro_right
-                  exact ht.left
-                }
-                { apply Exists.intro x
-                  apply Exists.intro t
-                  apply And.intro
-                  exact hx
-                  apply And.intro
-                  exact ht.left
-                  trivial
-                }
-              }
-              { sorry }
-            }
-            { sorry }
-          }
-          { sorry }
-        }
-        { rw [Relation.Spec] at h
-          obtain ⟨_, h⟩ := h
-          rw [Set.relation_condition] at h
-          obtain ⟨x, y, hx, hy, ht, hxyeq⟩ := h
-          obtain ⟨t, ⟨ht, ht₂, ht₁⟩⟩ := ht
-          apply Exists.intro x
-          apply Exists.intro y
-          apply Exists.intro t
-          apply And.intro
-          { rw [IsFunction] at hG
-            rw [hG.left, Relation.Spec]
-            apply And.intro
-            { aesop }
-            { rw [Set.relation_condition]
-              apply Exists.intro x
-              apply Exists.intro t
-              apply And.intro
-              exact hx
-              apply And.intro
-              exact ht
-              apply And.intro
-              exact ht₂
-              trivial
-            }
-          }
-          apply And.intro
-          { rw [IsFunction] at hF
-            obtain ⟨hF, _⟩ := hF
-            rw [hF, Relation.Spec]
-            apply And.intro
-            { rw [Product.Spec]
-              apply And.intro
-              { apply OrderedPair.in_power_power
-                rw [Union.Spec]
-                apply Or.intro_left
-                exact ht
-                rw [Union.Spec]
-                apply Or.intro_right
-                exact hy
-              }
-              { apply Exists.intro t
-                apply Exists.intro y
-                apply And.intro
-                exact ht
-                apply And.intro
-                exact hy
-                trivial
-              }
-            }
-            { rw [Set.relation_condition]
-              apply Exists.intro t
-              apply Exists.intro y
-              apply And.intro
-              exact ht
-              apply And.intro
-              exact hy
-              apply And.intro
-              exact ht₁
-              trivial
-            }
-          }
-          { trivial }
-        }
-      }
-    }
-    { intro x hx
-      rw [Relation.Domain.Spec] at hx
-      obtain ⟨y, hy⟩ := hx
+  theorem inverse_single_rooted (F : Set) : IsFunction (Inverse F) ↔ SingleRooted F := by
+    apply Iff.intro
+    { intro hFi
+      rw [IsFunction, domain_inverse] at hFi
+      obtain ⟨_, hFi⟩ := hFi
+      rw [SingleRooted]
+      intro x hx
+      have hy := hFi x hx
+      obtain ⟨y, hy, hy'⟩ := hy
+      rw [Inverse.Spec] at hy
+      obtain ⟨u, v, huv⟩ := hy
+      have huveq : x = v ∧ y = u := by
+        rw [OrderedPair.uniqueness] at huv
+        exact huv.right
+      rw [←huveq.right, ←huveq.left] at huv
       apply Exists.intro y
       apply And.intro
+      { exact huv.left }
       { aesop }
-      { intro y' hy'
-        -- There is a unique t such that xGt
-        -- There is a unique t' such that tFt'
-        rw [Composition.Spec] at hy
-        obtain ⟨hxy, ⟨u', v', t, hxt, hty, heq⟩⟩ := hy
-        rw [OrderedPair.uniqueness] at heq
-        rw [←heq.left] at hxt
-        rw [←heq.right] at hty
-
-        rw [Composition.Spec] at hy'
-        obtain ⟨hxy', ⟨u', v', t', hxt', hty', heq⟩⟩ := hy'
-        rw [OrderedPair.uniqueness] at heq
-        rw [←heq.left] at hxt'
-        rw [←heq.right] at hty'
-
-        have hteq : t = t' := by
-          apply Set.function_functional
-          apply hG
-          apply hxt
-          exact hxt'
-        subst hteq
-        apply Set.function_functional
-        apply hF
-        apply hty'
-        exact hty
-      }
     }
+    { intro h
+      sorry
+    }
+  theorem relation_function_single_rooted (F : Set) {hF : IsRelation F} : IsFunction F ↔ SingleRooted (Inverse F) := by sorry
 
+  /-
+  [Enderton, Theorem 3G, p. 46]
+  Assume that F is a one-to-one function. If x ∈ dom F, then F⁻¹(F(x)) = x. If y ∈ ran F, then F(F⁻¹(y)) = y.
+  -/
+  theorem one_to_one_inverse (F : Set) : IsFunction F → (∀ x, x ∈ (dom F) → ∃ y, ⟨x, y⟩ ∈ F ∧ ⟨y, x⟩ ∈ F⁻¹) := by sorry
+  theorem one_to_one_inverse' (F : Set) : IsFunction F → (∀ y, y ∈ (ran F) → ∃ x, ⟨y, x⟩ ∈ F⁻¹ ∧ ⟨x, y⟩ ∈ F) := by sorry
 end Set
